preservation.v
@@ -6,6 +6,7 @@ Require Import sframe.
 Require Import reductions.
 Require Import typing.
 Require Import namesAndTypes.
+Require Import wf_env.
 
 Import ConcreteEverything.
 
@@ -16,24 +17,189 @@ Section Preservation.
   Definition subtypeP := subtype P.
   Definition fldP := fld P.
   Definition ftypeP := ftype P.
-
-  Print sigT.
-
-  Print snd.
-  Print pair.
-
+  
   Theorem preservation_light :
     forall gamma H H' L L' t t' sigma eff,
       Reduction_SF ( # H, L, t !)
                    ( # H', L', t' !)
       ->
       TypeChecks gamma eff t sigma ->
-      {sig_gam : prod typecheck_type Gamma_type  & TypeChecks (snd sig_gam) eff t' (fst sig_gam)}.
+      {Gamma' : Gamma_type & TypeChecks Gamma' eff t' sigma}.
     intros.
     case_eq t; intros;  rewrite H0 in *  ;    clear H0 t; inversion X;
     inversion X0;
-      exists (sigma , p_gamma.updatePartFunc gamma v sigma0); cbn;
+      exists (p_gamma.updatePartFunc gamma v sigma0); cbn;
       rewrite H9 in *; auto.
   Qed.
 
-  
+  Theorem single_frame_WF_ENV_preservation :
+    forall H H' L L' t t' sigma ann,
+      WF_Frame H (ann_frame (sframe L t) ann) sigma ->
+      Reduction_SF ( # H, L, t !) ( # H', L', t' !) ->
+      WF_Frame H (ann_frame (sframe L' t') ann) sigma.
+    intros.
+    case_eq t; intros;   rewrite H0 in *  ;    clear H0 t;   inversion X0.
+
+    inversion X0.
+    rewrite <- H18 in *; clear H18 H12 H7 H1.
+    rewrite <- H19 in *; clear H19 H13 H2.
+    rewrite <- H6 in *; rewrite <- H9 in *. clear H20 H17 H9 H6.
+    clear H14.
+    rewrite <- H5 in *.
+    inversion H16.
+    rewrite H2 in *; clear H2 H16 H5.
+    rewrite <- H4 in *.
+    clear H15 H4 v.
+    clear L1 H11 t0 y0 x0.
+    assert (Some null_ref_box0 = Some null_ref_box). transitivity (p_env.func L y).
+    auto. auto.
+    inversion H1.
+    rewrite H4 in *.
+    clear H4 H1 H8 H21 null_ref_box0.
+
+    inversion X.
+    clear H6 t0. clear H4 H1. clear L1 H2.
+    clear ann0 sigma0 H7 H5.
+    clear H' t' e0 e L' H0.
+    
+    inversion X1.
+    clear gamma H0 x0 H4 eff0 H1 t0 H6 H2 tau H5 e.
+    apply (t_frame1 H (p_gamma.updatePartFunc Gamma x sigma0) eff t
+                    (p_env.updatePartFunc L x null_ref_box) ann sigma H3).
+    apply X4.
+    split.
+    destruct X2.
+    apply (subset_preserved _ _ _ _ _ g).
+    intros.
+    elim (v_eq_dec x x0).
+    intro; rewrite <- a in *; clear a.
+
+    inversion X3.
+    clear H6 H4 H1; rewrite <- H2 in *; clear H2 sigma2.
+    set (wf_var_y := snd X2 y sigma0 H5).
+    
+    (* 3.
+     *)
+    induction null_ref_box.
+    (* 
+     * 3. (a), L(y) = null
+     *)
+    apply inl; apply inl.
+    apply (proj1 (p_env.updatedFuncProp L x envNull x) (eq_refl x)).
+
+    (* 3. (b), L(y) = o*)
+    rename r into o.
+    rename H10 into _3_b_i_A. 
+    induction  wf_var_y.
+    induction a. (* case L(y) = null in WF-var *)
+    rewrite a in _3_b_i_A; discriminate.
+
+    induction b;  destruct x2. (* case L(y) = o', H(o') = <C, FM> in WF-var*)
+    induction p.
+    destruct p.
+    rewrite (_3_b_i_A) in *; inversion H1.
+    destruct H2.
+    rewrite ->  H6 in *.
+    clear o H6.
+    rename r into o. (* it couldn't do it directly *)
+    rename c into C'.
+    clear H1.
+
+    apply inl. apply inr.
+    exists (C', o).
+    exists x2.
+    split.
+    apply p_env.updatedFuncProp; apply eq_refl.
+    split.
+
+    set (lem := proj1 (p_gamma.updatedFuncProp gamma  x sigma0 x) (eq_refl x)).
+    rewrite lem in H0; inversion H0; rewrite H6 in *.
+    rename sigma1 into sigma'; clear H6 H0.
+    rewrite H2 in H5; inversion H5; rewrite <- H1 in *.
+    clear H1 sigma'.
+    apply p_gamma.updatedFuncProp; apply eq_refl.
+    auto.
+
+    induction b; destruct x2; induction p; destruct p; destruct H2.
+
+    rewrite (_3_b_i_A) in *; inversion H1.
+    (* destruct H2. *)
+    rewrite ->  H7 in *.
+    clear o H7.
+    rename r into o. (* it couldn't do it directly *)
+    rename c into C'.
+    clear H1.
+
+    apply inr.
+    exists (C', o).
+    exists x2.
+    split.
+    apply p_env.updatedFuncProp; apply eq_refl.
+    split.
+
+    set (lem := proj1 (p_gamma.updatedFuncProp gamma  x sigma0 x) (eq_refl x)).
+    rewrite lem in H0; inversion H0. rewrite H6 in *.
+    rename sigma1 into sigma'; clear  H6 H0.
+    rewrite H2 in H5; inversion H5; rewrite <- H1 in *.
+    clear H1 H5.
+    exact lem.
+    exact H4.
+
+    (* 3 c, L(y) = b(o)*)
+    rename H10 into _3_c.
+    rename r into o.
+    destruct X2 as [_3_c_i_A _3_c_i_B].
+    clear Gamma.
+    rename H5 into _1_b.
+    rename sigma0 into sigma'.
+    simpl in wf_var_y.
+
+    rename wf_var_y into _3_c_ii.
+    induction (_3_c_ii).
+    induction a. (* 3. c. iii. *)
+    rewrite a in _3_c; discriminate. (* 3. c. iv.*)
+    induction b; destruct x2; destruct p; destruct a.
+    rename H1 into _3_c_v.
+    rewrite _3_c_v in _3_c; discriminate. (* 3. c. v. *)
+
+    
+
+    destruct b; destruct x2. destruct y0; destruct a; destruct H2.
+    rewrite _3_c in H1; inversion H1.
+    rename x0 into z.
+    rename sigma1 into tau.
+    intro.
+
+    assert (p_gamma.func Gamma z = Some tau) as _4_a.
+    rewrite <- H0.
+    symmetry.
+    apply p_gamma.updatedFuncProp. firstorder.
+    TODO: finish here!
+    (* assert (p_gamma.func Gamma z = Some tau) as _4_a. *)
+    
+    
+    (* destruct b; destruct x2. destruct y0; destruct a; destruct H2. *)
+    (* rewrite _1_b in H2; inversion H2. *)
+    (* rewrite  H6 in *. *)
+    (* clear H2. *)
+    (* assert (p_gamma.func gamma y = Some (typt_box c)). *)
+    (* transitivity (Some sigma'). auto. *)
+    (* f_equal. auto. *)
+    (* rename H2 into _1_b'. *)
+    (* set (_3_c_ii' := _3_c_i_B y (typt_box c) _1_b'). *)
+    (* clear _3_c_ii _1_b. *)
+    (* rename _1_b' into _3_c_vi_A. *)
+    (* rename H4 into _3_c_vi_B. *)
+    (* rename _3_c_ii' into _3_c_ii. *)
+    (* clear H6 sigma'. *)
+    (* rewrite _3_c in H1. *)
+    
+    
+    
+    set (_1_b' := )
+    rewrite H6 in _3_c_ii.
+    
+    rewrite <- H7 in *.
+    set (test := _3_c_i_B x )
+    apply p_gamma.updatedFuncProp; apply eq_refl.
+    auto.
