wf_env.v
@@ -1,0 +1,132 @@
+Require Import syntax.
+Require Import partial.
+Require Import heap.
+Require Import classTable.
+Require Import sframe.
+Require Import reductions.
+Require Import typing.
+Require Import namesAndTypes.
+
+Import ConcreteEverything.
+
+Section WF_Env.
+
+  Import Coq.Lists.List.
+
+  Definition gamma_env_subset (gamma: Gamma_type) (L: Env_type) :=
+    forall x,
+      In x (p_gamma.domain gamma) ->
+      In x (p_env.domain L).
+
+  Theorem in_dec_equivalence (A: Type) (eq_dec: forall (x y: A),
+                                                 {x = y} + {x <> y}
+                                      ) :
+    forall x l1 l2,
+      (@In A x l1 <-> In x l2) <-> (~ In x l1 <-> ~ In x l2).
+    intros.
+    set (leml1 := in_dec eq_dec x l1).
+    set (leml2 := in_dec eq_dec x l2).
+    firstorder.
+  Defined.
+    
+
+  Theorem subset_preserved gamma L x sigma envVal :
+    gamma_env_subset gamma L ->
+    gamma_env_subset (p_gamma.updatePartFunc gamma x sigma )
+                     (p_env.updatePartFunc L x envVal).
+    intros subset x'.
+    intro.
+    set (lem_gamma := p_gamma.updatedFuncProp gamma x sigma x').
+    set (lem_env := p_env.updatedFuncProp L x envVal x').
+    
+    elim (v_eq_dec x' x).
+    intro; rewrite a in *; clear a.
+    set (lem_env_x := (proj1 lem_env) (eq_refl x)).
+    set (lem_upd_env := proj1 (p_env.fDomainCompat (p_env.updatePartFunc L x envVal) x)).
+    set (in_or_not := in_dec v_eq_dec x (p_env.domain (p_env.updatePartFunc L x envVal))).
+    elim in_or_not.
+    auto.
+    intro.
+    set (not_in := lem_upd_env b).
+    rewrite not_in in lem_env_x; discriminate.
+
+    (* x != x'
+     * Proof structure:
+     *    Then x' in dom(Gamma) <--> x' in dom(Gamma[x |-> sigma])
+     *         x' in dom(L) <--> x' in dom(L[x |-> envVal])
+     *)
+    intro x_neq.
+    assert (In x' (p_gamma.domain gamma) <-> In x' (p_gamma.domain
+                                                      (p_gamma.updatePartFunc gamma x sigma))).
+    apply (proj2 (in_dec_equivalence p_gamma.A v_eq_dec x' _ _)).
+    set (lem_gamma' := (proj2 lem_gamma) x_neq).
+    set (lem_gamma_upd_equiv
+         := proj2 (p_gamma.fDomainCompat (p_gamma.updatePartFunc gamma x sigma) x')).
+    set (lem_gamma_equiv := proj2 (p_gamma.fDomainCompat gamma x')).
+    firstorder.
+
+    assert (In x' (p_env.domain L) <-> In x' (p_env.domain
+                                                      (p_env.updatePartFunc L x envVal))).
+    apply (proj2 (in_dec_equivalence p_env.A v_eq_dec x' _ _)).
+    set (lem_env' := (proj2 lem_env) x_neq).
+    set (lem_env_upd_equiv
+         := proj2 (p_env.fDomainCompat (p_env.updatePartFunc L x envVal) x')).
+    set (lem_env_equiv := proj2 (p_env.fDomainCompat L x')).
+    firstorder.
+    firstorder.    
+  Qed.
+    
+        
+    
+
+  Import Coq.Lists.List.
+
+  Definition heap_typeof (H: Heap_type) (o: Ref_type)
+             (witn: In o (p_heap.domain H)) :
+    ClassName_type.
+    set (lem := proj2 (p_heap.fDomainCompat H o)).
+    case_eq (p_heap.func H o).
+    intros;    destruct b;    exact c.
+    intro is_none; set (is_absurd := lem is_none); auto.
+  Defined.
+
+  Parameter P: Program.
+
+  
+  Definition subtypeP := subtype P.
+
+  Local Open Scope type_scope.
+
+  
+  Definition WF_Var (H: Heap_type) (Gamma: Gamma_type) (L: Env_type) (x: VarName_type):=
+    (p_env.func L x = Some envNull) +
+    {C_o |
+     match C_o with
+       | (C, o) => {witn |
+                    p_env.func L x = Some (envRef o) /\
+                    p_gamma.func Gamma x = Some (typt_class C) /\
+                    subtypeP (typt_class (heap_typeof H o witn)) (typt_class C)
+                   }
+     end} +
+    {C_o |
+     match C_o with
+       | (C, o) => {witn |
+                    p_env.func L x = Some (envRef o) /\
+                    p_gamma.func Gamma x = Some (typt_box C) /\
+                    subtypeP (typt_class (heap_typeof H o witn)) (typt_class C)
+                   }
+     end}.
+
+  Definition WF_Env H Gamma L :=
+    gamma_env_subset Gamma L *
+    forall x sigma,
+      p_gamma.func Gamma x = Some sigma ->
+      WF_Var H Gamma L x.
+
+  Inductive WF_Frame : Heap_type -> ann_frame_type -> typecheck_type -> Type :=
+  | t_frame1 : forall H Gamma eff t L ann sigma,
+                isTerm t ->
+                TypeChecks Gamma eff t sigma ->
+                WF_Env H Gamma L ->
+                WF_Frame H (ann_frame (sframe L t) ann) sigma.
+End WF_Env.
